

# CONTROL SYSTEMS

D.TEJASRI

ES17BTECH11007

February 2020

## Problem Statement

Consider the following state-space representation of a linear time-invariant system  $\dot{x}(t) = \begin{bmatrix} 1 & 0 \\ 0 & 2 \end{bmatrix} x(t)$  ;

$$y(t) = c^T x(t) ;$$

$$c = \begin{bmatrix} 1 \\ 1 \end{bmatrix} \text{ and } x(0) = \begin{bmatrix} 1 \\ 1 \end{bmatrix} ;$$

The value of  $y(t)$  for  $t = \log_e 2$  is

Given  $\dot{x}(t) = \begin{bmatrix} 1 & 0 \\ 0 & 2 \end{bmatrix} x(t)$

also we know that  $\dot{x}(t) = Ax(t)$

on comparing we get  $A = \begin{bmatrix} 1 & 0 \\ 0 & 2 \end{bmatrix}$ ;

now  $y(t) = c^T x(t)$  ;  $x(t) = e^{At}x(0)$ ;

where  $e^{At} = L^{-1}[(sI - A)^{-1}]$ ;

$$sI - A = \begin{bmatrix} s-1 & 0 \\ 0 & s-2 \end{bmatrix}$$

$$(sI - A)^{-1} = \begin{bmatrix} \frac{1}{s-1} & 0 \\ 0 & \frac{1}{s-2} \end{bmatrix}$$

$$e^{At} = \begin{bmatrix} e^t & 0 \\ 0 & e^{2t} \end{bmatrix}$$

$$x(t) = \begin{bmatrix} e^t & 0 \\ 0 & e^{2t} \end{bmatrix} \begin{bmatrix} 1 \\ 1 \end{bmatrix} = \begin{bmatrix} e^t \\ e^{2t} \end{bmatrix}$$

$$y(t) = \begin{pmatrix} 1 \\ 1 \end{pmatrix} \begin{bmatrix} e^t \\ e^{2t} \end{bmatrix} = [e^t + e^{2t}]$$

now for  $t = \log_e 2$

$$y(t) = [e^{\log_e 2} + e^{2\log_e 2}]$$

$$= [2 + 4] = 6$$

$$y(t) = 6$$